\documentclass[12pt,oneside,a4paper]{article}
\usepackage[T1]{fontenc}
\usepackage[utf8]{inputenc}
\usepackage[nofoot,hdivide={1cm,*,1cm},vdivide={1cm,*,1cm}]{geometry}
\usepackage{hyperref}
\usepackage{amsmath}
\usepackage{amssymb}
\usepackage{amsthm}
\usepackage{listings}
\usepackage{graphicx}
\usepackage{color}
\definecolor{lbcolor}{rgb}{0.95,0.95,0.95}  

\lstset
 {
    language = python,
    columns  = flexible,
    xleftmargin = 0.5cm,
    backgroundcolor=\color{lbcolor},  
 }




\author{Wojciech Adamiec}
\title{
    \textbf{RPIS - List 7 Task 6}\\
}

\renewcommand{\qedsymbol}{$\blacksquare$}
\newcommand\numeq[1]%
  {\stackrel{\scriptscriptstyle \mkern-1.5mu#1\mkern-1.5mu }{=}}

\begin{document}
\maketitle

\paragraph{Prove that:}\

$$\sum^n_{k=1}{(X_k - \mu)^2} = \sum^n_{k=1}{(X_k - \bar{X})^2} + n(\bar{X}-\mu)^2$$

\begin{proof}
$$\sum^n_{k=1}{(X_k - \mu)^2} = \sum^n_{k=1}{(X_k - \bar{X} + \bar{X}- \mu)^2} =$$
$$= \sum^n_{k=1}{((X_k - \bar{X})^2 + (\bar{X}- \mu)^2 + 2(X_k - \bar{X})(\bar{X}-\mu))} =$$
$$=\sum^n_{k=1}{(X_k - \bar{X})^2} + n(\bar{X}- \mu)^2 + 2(\bar{X}-\mu)\sum^n_{k=1}(X_k - \bar{X}) =$$
$$ \sum^n_{k=1}{(X_k - \bar{X})^2 + n(\bar{X}- \mu)^2 + 2(\bar{X}-\mu)(\sum^n_{k=1}X_k - \sum^n_{k=1}\bar{X})}=$$
$$= \sum^n_{k=1}{(X_k - \bar{X})^2} + n(\bar{X}- \mu)^2 + 2(\bar{X}-\mu)(n \cdot \frac{1}{n} \cdot \sum^n_{k=1}X_k - n\bar{X}) =$$
$$= \sum^n_{k=1}{(X_k - \bar{X})^2} + n(\bar{X}- \mu)^2 + 2(\bar{X}-\mu)\cdot 0 =$$
$$= \sum^n_{k=1}{(X_k - \bar{X})^2} + n(\bar{X} - \mu)^2$$
\end{proof}

\end{document}
